test/SimplMatchTest.v
@@ -1,0 +1,87 @@
+(*Here we have a small test for simplifying
+  pattern matches.
+  In particular, we define an option type and have the function
+  foo (l: option 'a) : int =
+  match l with
+  | None -> 0
+  | Some _ -> 1
+  end
+  
+  and we prove that
+  1. foo None = 0
+  2. foo (Some x) = 1 for any x
+
+  (we don't do with prop because we didn't implement predicate
+    unfolding yet, though we could easily)
+  *)
+Require Import Tactics.
+From mathcomp Require Import all_ssreflect.
+Set Bullet Behavior "Strict Subproofs".
+
+Module SimplMatchTest.
+
+Local Open Scope string_scope.
+
+Definition zero : term := Tconst (ConstInt 0).
+Definition one : term := Tconst (ConstInt 1).
+
+(*First, define option type (we will do for real later)*)
+(*TODO: make this nicer*)
+Definition avar : typevar := "a".
+Definition a : vty := vty_var avar.
+Definition option_ts : typesym := mk_ts "option" [avar].
+Definition option_ty : vty := vty_cons option_ts [a].
+Definition none_fs : funsym := funsym_noty "None" nil option_ty.
+Definition some_fs : funsym := funsym_noty "Some" [a] option_ty.
+Definition option_adt : alg_datatype := alg_def option_ts 
+  (list_to_ne_list [none_fs; some_fs] Logic.eq_refl).
+Definition option_mut: mut_adt := mk_mut [option_adt] [avar] erefl.
+
+(*Our function definition*)
+Definition isSome : funsym := funsym_noty "isSome" [option_ty] vty_int.
+Definition o: vsymbol := ("o", option_ty).
+Definition isSome_def : funpred_def :=
+  fun_def isSome [o] 
+  (Tmatch (Tvar o) option_ty
+    [(Pconstr none_fs [a] nil, zero) (*None -> 0*);
+     (Pconstr some_fs [a] [Pwild], one) (*Some _ -> 1*)]).
+
+Definition none : term := Tfun none_fs [a] nil.
+Definition some y : term := Tfun some_fs [a] [y].
+
+(*Define a variable x of type a*)
+Definition x : vsymbol := ("x", a).
+
+Definition simpl_match_theory : theory :=
+  rev [
+    tdef (datatype_def option_mut);
+    tdef (recursive_def [isSome_def]);
+    tprop Pgoal "isSome_None" (Feq vty_int
+      (Tfun isSome [a] [none]) zero);
+    tprop Pgoal "isSome_some" (Fquant Tforall x
+      (Feq vty_int (Tfun isSome [a] [some (Tvar x)])
+        one))
+  ].
+
+Lemma simpl_match_theory_typed : typed_theory simpl_match_theory.
+Proof.
+  check_theory.
+Qed.
+
+Lemma simpl_match_theory_valid: valid_theory simpl_match_theory.
+Proof.
+  simpl. split_all; auto.
+  - exists ["a"].
+    wstart.
+    wintros "x".
+    wunfold isSome.
+    wsimpl_match.
+    wreflexivity.
+  - exists ["a"].
+    wstart.
+    wunfold isSome.
+    wsimpl_match.
+    wreflexivity.
+Qed.
+
+End SimplMatchTest.
